EffectSSA/Semantics/TEnvironment.lean
@@ -1,0 +1,90 @@
+import EffectSSA.Syntax.Typed
+import EffectSSA.Semantics.Program
+import EffectSSA.Semantics.Lemmas
+
+/-!
+# Intrinsically Typed Environments
+-/
+namespace EffectSSA
+variable {τ} [MemoryModel τ]
+
+structure Semantics.TEnvironment (Γ : Context τ) where
+  env : Environment τ
+  wt : env.WellTyped Γ := by grind
+
+/-!
+### Grind
+-/
+open Semantics (TEnvironment)
+
+grind_pattern TEnvironment.wt => TEnvironment.env self
+
+
+/-!
+## Coercions
+--------------------------------------------------------------------------------
+The typed structures can be implicitly coerced into the underlying
+untyped variants
+-/
+open Semantics (Environment TEnvironment)
+variable {Γ : Context τ}
+
+instance : CoeOut (TEnvironment Γ) (Environment τ) where coe := TEnvironment.env
+instance : CoeOut (TVar Γ t) Var where coe := TVar.toVar
+
+instance : CoeOut (TEnvironment Γ × α) (Environment τ × α) where
+  coe p := (p.1.env, p.2)
+
+/-!
+## Definitions
+--------------------------------------------------------------------------------
+-/
+namespace Semantics.TEnvironment
+
+def get (env : TEnvironment Γ) (v : TVar Γ t) : τ.TVal t :=
+  env.env.getAs? v.toVar t |>.get <| by
+    have := env.wt v
+    grind
+
+/--
+Limit a typed environment to the given variables, yielding a smaller
+-/
+def limitTo (env : TEnvironment Γ) (vs : TVarList Γ ts) : TEnvironment ⟨ts⟩ where
+  env := .ofList <| vs.map (env.get · |>.toVal)
+  wt := by grind [Environment.getAs?, Environment.get?]
+
+/-- Empty environment. -/
+instance : EmptyCollection (TEnvironment (τ:=τ) ∅) where
+  emptyCollection := { env := ∅ }
+
+end Semantics.TEnvironment
+
+/-!
+## Lemmas
+--------------------------------------------------------------------------------
+-/
+
+namespace Semantics.TEnvironment
+variable {Γ : Context τ} (env : TEnvironment Γ)
+
+@[simp, grind =] theorem env_getAs?_isSome_eq :
+    (env.env.getAs? v t).isSome = decide (Γ[v]? = some t) := by
+  simp [env.wt v t]
+
+@[simp, grind =] theorem env_getAs?_isSome :
+    (env.env.getAs? v t).isSome ↔ Γ[v]? = some t := by
+  simp
+
+@[simp, grind =] theorem env_getAs?_eq (h : Γ[v]? = some t) (env : TEnvironment Γ) :
+    (env.env.getAs? v t) = some (env.get ⟨v, h⟩) := by
+  simp [get]
+@[simp, grind =] theorem env_getAs_eq (h : Γ[v]? = some t) (env : TEnvironment Γ) :
+    (env.env.getAs v t) = some (env.get ⟨v, h⟩) := by
+  simp [get, Environment.getAs]
+
+@[simp, grind =] theorem env_empty : TEnvironment.env (τ:=τ) (∅ : TEnvironment ∅) = ∅ := by rfl
+
+@[simp, grind =] theorem env_limitTo? (vs : TVarList Γ ts) :
+    env.env.limitTo? vs.toList = some (env.limitTo vs).env := by
+  -- FIXME: this should eventually be proven
+  sorry
