EffectSSA/Semantics/TProgram.lean
@@ -1,0 +1,137 @@
+import EffectSSA.Syntax.Typed
+import EffectSSA.Semantics.Program
+import EffectSSA.Semantics.Lemmas
+import EffectSSA.Semantics.TEnvironment
+
+/-!
+# Semantics of Intrinsically Typed Programs
+This file uses the untyped semantics to define semantics for intrinsically
+well-typed programs. This is particularly useful, since the welltypedness
+means these semantics can never return a type error.
+-/
+namespace EffectSSA
+variable {τ} [MemoryModel τ] {Γ Δ : Context τ}
+
+open Semantics (Environment TEnvironment)
+
+/-!
+## Instruction
+--------------------------------------------------------------------------------
+-/
+
+@[grind <=]
+theorem Instruction.isSome_exec {i : Instruction τ} {env : Environment τ}
+    (wt_i : i.WellTyped Γ Δ) (wt_env : env.WellTyped Γ) :
+    (i.exec env es).isSome := by
+  obtain ⟨env, rfl⟩ : ∃ (env' : TEnvironment _), env = env' := ⟨⟨env, wt_env⟩, rfl⟩
+  clear wt_env
+  unfold exec execM
+  cases wt_i <;> (simp; (repeat rw [TEnvironment.env_getAs_eq (by assumption)]); try grind)
+  next => simp
+
+def TInstruction.exec (i : TInstruction Γ Δ) (env : TEnvironment Γ) (es : Option (Trace τ)) :
+    TEnvironment Δ × (Option (Trace τ)) :=
+  let res := (i.instruction.exec env.env es).get <| Instruction.isSome_exec i.wt env.wt
+  have wt := by
+    subst res
+    cases i
+    · simp [Instruction.exec, Instruction.execM]; grind
+    · simp [Instruction.exec, Instruction.execM]; grind
+    · simp [Instruction.exec, Instruction.execM]; sorry
+    · simp [Instruction.exec, Instruction.execM]; sorry
+    · simp [Instruction.exec, Instruction.execM]; grind
+    · simp [Instruction.exec, Instruction.execM]; grind
+  ⟨⟨res.1, wt⟩, res.2⟩
+
+@[grind =>]
+theorem Instruction.exec_eq_of_wellTyped {i : Instruction τ} {env : Environment τ}
+    (wt_i : i.WellTyped Γ Δ) (wt_env : env.WellTyped Γ) (es?) :
+    i.exec env es? = some (TInstruction.exec ⟨i, wt_i⟩ ⟨env, wt_env⟩ es?) := by
+  simp [TInstruction.exec]
+
+@[simp, grind =]
+theorem TInstruction.exec_instruction_eq {i : TInstruction Γ Δ} {env : TEnvironment Γ} :
+    i.instruction.exec env.env es? = some (i.exec env es?) := by
+  rw [Instruction.exec_eq_of_wellTyped]
+
+/-!
+## InstructionSeq
+-/
+
+@[grind! <=]
+theorem InstructionSeq.isSome_exec {is : InstructionSeq τ} {env : Environment τ}
+    (wt_is : is.WellTypedWith Γ Δ) (wt_env : env.WellTyped Γ) :
+    (is.exec env es).isSome := by
+  obtain ⟨env, rfl⟩ : ∃ (env' : TEnvironment _), env = env' := ⟨⟨env, wt_env⟩, rfl⟩
+  obtain ⟨is, rfl⟩ : ∃ (is' : TInstructionSeq _ _), is = is' := ⟨⟨is, wt_is⟩, rfl⟩
+  clear wt_env wt_is
+  induction is generalizing es <;> simp [*]
+
+def TInstructionSeq.exec (is : TInstructionSeq Γ Δ) (env : TEnvironment Γ) (es? : Option (Trace τ)) :
+    TEnvironment Δ × Option (Trace τ) :=
+  let res := (is.seq.exec env es?).get <| InstructionSeq.isSome_exec is.wt env.wt
+  have wt := by intro v t; induction is generalizing es? <;> grind
+  ⟨⟨res.1, wt⟩, res.2⟩
+
+
+@[grind =>]
+theorem InstructionSeq.exec_eq_of_wellTyped {is : InstructionSeq τ} {env : Environment τ}
+    (wt_i : is.WellTypedWith Γ Δ) (wt_env : env.WellTyped Γ) (es?) :
+    is.exec env es? = some (TInstructionSeq.exec ⟨is, wt_i⟩ ⟨env, wt_env⟩ es?) := by
+  simp [TInstructionSeq.exec]
+
+@[simp, grind =]
+theorem TInstructionSeq.exec_instruction {is : TInstructionSeq Γ Δ} {env : TEnvironment Γ} :
+    is.seq.exec env.env es? = some (is.exec env es?) := by
+  rw [InstructionSeq.exec_eq_of_wellTyped]
+
+/-!
+## Program
+-/
+
+@[grind <=] theorem Program.isSome_exec {p : Program τ} {env : Environment τ}
+    (wt_p : p.WellTyped Γ ts) (wt_env : env.WellTyped Γ) :
+    (p.exec env es).isSome := by
+  obtain ⟨env, rfl⟩ : ∃ (env' : TEnvironment _), env = env' := ⟨⟨env, wt_env⟩, rfl⟩
+  obtain ⟨p, rfl⟩ : ∃ (p' : TProgram _ _), p = p' := ⟨⟨p, wt_p⟩, rfl⟩
+  simp [exec, execM]
+
+def TProgram.exec (p : TProgram Γ ts) (env : TEnvironment Γ) (es? : Option (Trace τ)) :
+    TEnvironment ⟨ts⟩ × Option (Trace τ) :=
+  let res := (p.program.exec env es?).get <| Program.isSome_exec p.wt env.wt
+  have wt := by
+    simp [res, Environment.WellTyped, Program.exec, Program.execM]
+  ⟨⟨res.1, wt⟩, res.2⟩
+
+@[grind] def TProgram.execClosed (p : TProgram (τ:=τ) ∅ ts) :
+    TEnvironment ⟨ts⟩ × Option (Trace τ) :=
+  p.exec ∅ (some ∅)
+
+section Lemmas
+
+@[grind =>]
+theorem Program.exec_eq_of_wellTyped {p : Program τ} {env : Environment τ}
+    (wt_p : p.WellTyped Γ ts) (wt_env : env.WellTyped Γ) (es?) :
+    p.exec env es? = some (TProgram.exec ⟨p, wt_p⟩ ⟨env, wt_env⟩ es? : Environment τ × _) := by
+  simp [TProgram.exec]
+
+@[simp, grind =]
+theorem TProgram.exec_program {p : TProgram Γ ts} {env : TEnvironment Γ} :
+    p.program.exec env.env es? = some (p.exec env es? : Environment τ × _) := by
+  simp [Program.exec_eq_of_wellTyped p.wt env.wt]
+
+
+@[simp, grind =] theorem TProgram.execClosed_program {p : TProgram (τ:=τ) ∅ ts} :
+    p.program.execClosed = some (p.execClosed : Environment τ × _) := by
+  have : (∅ : Environment τ) = (∅ : TEnvironment (τ:=τ) ∅) := rfl
+  simp only [Program.execClosed, this, TProgram.exec_program]
+  rfl
+
+@[simp] theorem Program.execClosed_eq_of_wellTyped {p : Program τ}
+    (wt : p.WellTyped ∅ ts):
+    p.execClosed = some (TProgram.execClosed ⟨p, wt⟩ : Environment τ × _) := by
+  generalize hp : TProgram.mk p wt = p'
+  have : p = p'.program := by grind
+  grind
+
+end Lemmas
